fix last admitted

theories/coroutine.v
@@ -20,15 +20,39 @@ Definition yield_addr : Z := 2000.
 
 Definition coro_state_addr : Z := 3000.
 
-Definition coro_saved_regs : list string := "PC"::saved_registers.
+Definition coro_saved_regs : list string := saved_registers ++ ["PC"].
+Lemma coro_saved_regs_length :
+  length coro_saved_regs = 13%nat.
+Proof. done. Qed.
+Lemma coro_saved_regs_lookup_saved i :
+  (i < 12)%nat →
+  coro_saved_regs !! i = Some (saved_registers !!! i).
+Proof. move => ?. do 12 (destruct i as [|i]; try done); lia. Qed.
+Lemma coro_saved_regs_take_PC r :
+  r ≠ "PC" →
+  r ∈ take 12 coro_saved_regs ↔ r ∈ coro_saved_regs.
+Proof. set_solver. Qed.
+Lemma coro_saved_regs_take_saved r i :
+  (i < 12)%nat →
+  r ≠ saved_registers !!! i →
+  r ∈ take (i + 1) coro_saved_regs ↔ r ∈ take i coro_saved_regs.
+Proof. cbn. repeat (destruct i as [|i] => /=; [set_solver|try lia]). Qed.
 
 Definition coro_get_regs (regs : gmap string Z) : list Z :=
   ((regs !!!.) <$> coro_saved_regs).
 Arguments coro_get_regs : simpl never.
 
+Definition coro_regs_mem_n (regs : gmap string Z) (n : nat) : gmap Z (option Z) :=
+  map_seqZ coro_state_addr (Some <$> take n (coro_get_regs regs)).
+Arguments coro_regs_mem_n : simpl never.
+
 Definition coro_regs_mem (regs : gmap string Z) : gmap Z (option Z) :=
-  map_seqZ coro_state_addr (Some <$> coro_get_regs regs).
+  coro_regs_mem_n regs (length coro_saved_regs).
 Arguments coro_regs_mem : simpl never.
+
+Definition coro_regs_regs_n (regs : gmap string Z) (n : nat) : gmap string Z :=
+  list_to_map ((λ x, (x, regs !!! x)) <$> take n coro_saved_regs).
+Arguments coro_regs_regs_n : simpl never.
 
 Definition coro_regs_regs (regs : gmap string Z) : gmap string Z :=
   list_to_map ((λ x, (x, regs !!! x)) <$> coro_saved_regs).
@@ -60,8 +84,8 @@ Lemma coro_regs_regs_saved_preserved rs rs' rs'':
 Proof.
   move => Hp. rewrite /coro_regs_regs. cbn.
   rewrite -!insert_union_l left_id_L.
-  apply map_preserved_insert_r_not_in; [compute_done|].
   repeat (apply map_preserved_insert_r_in; [compute_done|]; split; [apply: Hp; compute_done|]).
+  apply map_preserved_insert_r_not_in; [compute_done|].
   apply map_preserved_nil'. compute_done.
 Qed.
 
@@ -90,7 +114,101 @@ Proof.
   rewrite -!insert_union_l left_id_L.
   by repeat (rewrite lookup_total_insert_ne; [|naive_solver]).
 Qed.
+
+Lemma coro_regs_regs_lookup_Some rs r v:
+  coro_regs_regs rs !! r = Some v ↔ r ∈ coro_saved_regs ∧ v = rs !!! r.
+Proof.
+  rewrite /coro_regs_regs.
+  cbn.
+  rewrite !lookup_insert_Some !lookup_empty !elem_of_cons elem_of_nil.
+  naive_solver.
+Qed.
 Opaque coro_saved_regs.
+
+Lemma coro_regs_regs_n_lookup_Some rs r v i:
+  coro_regs_regs_n rs i !! r = Some v ↔ r ∈ take i coro_saved_regs ∧ v = rs !!! r.
+Proof.
+  rewrite /coro_regs_regs_n.
+  rewrite -elem_of_list_to_map.
+  2: { rewrite -list_fmap_compose. apply NoDup_fmap.
+       2: { do 15 (destruct i as [|i]; [compute_done|]). compute_done. }
+       move => ?? /=?. done. }
+  rewrite elem_of_list_fmap. naive_solver.
+Qed.
+
+Lemma coro_regs_regs_lookup_None rs r:
+  coro_regs_regs rs !! r = None ↔ r ∉ coro_saved_regs.
+Proof. rewrite eq_None_not_Some /is_Some. setoid_rewrite coro_regs_regs_lookup_Some. naive_solver. Qed.
+
+Lemma coro_regs_regs_n_lookup_None rs r i:
+  coro_regs_regs_n rs i !! r = None ↔ r ∉ take i coro_saved_regs.
+Proof. rewrite eq_None_not_Some /is_Some. setoid_rewrite coro_regs_regs_n_lookup_Some. naive_solver. Qed.
+
+Lemma coro_get_regs_lookup_Some rs i v :
+  coro_get_regs rs !! i = Some v ↔ ∃ r, coro_saved_regs !! i = Some r ∧ v = rs !!! r.
+Proof. by rewrite /coro_get_regs list_lookup_fmap fmap_Some. Qed.
+
+Lemma coro_regs_mem_n_lookup_Some (k : nat) rs (i : nat) j  v:
+  i ≤ 13 →
+  j = coro_state_addr + k →
+  coro_regs_mem_n rs i !! j = Some (Some v) ↔
+    ∃ r, coro_saved_regs !! k = Some r ∧ k < i ∧ v = rs !!! r.
+Proof.
+  move => ??. subst.
+  rewrite /coro_regs_mem_n lookup_map_seqZ_Some list_lookup_fmap fmap_Some.
+  setoid_rewrite lookup_take_Some. setoid_rewrite coro_get_regs_lookup_Some.
+  have ->: Z.to_nat (coro_state_addr + k - coro_state_addr) = k by lia.
+  split => ?; destruct_all?; simplify_eq; split!; lia.
+Qed.
+
+Lemma coro_regs_mem_lookup_Some (k : nat) rs j  v:
+  j = coro_state_addr + k →
+  coro_regs_mem rs !! j = Some (Some v) ↔
+    ∃ r, coro_saved_regs !! k = Some r ∧ k < 13 ∧ v = rs !!! r.
+Proof. move => ?. rewrite /coro_regs_mem coro_regs_mem_n_lookup_Some //. Qed.
+
+Lemma coro_regs_mem_n_lookup_None rs i j:
+  coro_regs_mem_n rs i !! j = None ↔ j < coro_state_addr ∨ coro_state_addr + (i `min` 13) ≤ j.
+Proof.
+  rewrite /coro_regs_mem_n lookup_map_seqZ_None fmap_length take_length.
+  rewrite /coro_get_regs fmap_length coro_saved_regs_length. lia.
+Qed.
+
+Lemma coro_regs_mem_n_insert rs (i : nat) v r:
+  coro_saved_regs !! i = Some r →
+  <[coro_state_addr + i := Some v]> (coro_regs_mem_n rs i) =
+    coro_regs_mem_n (<[r := v]> rs) (i + 1).
+Proof.
+  move => Hk. move: (Hk) => /(lookup_lt_Some _ _ _). rewrite coro_saved_regs_length => ?.
+  apply map_eq => k.
+  destruct (decide (k = coro_state_addr + i)); simplify_map_eq.
+  - symmetry. eapply coro_regs_mem_n_lookup_Some; [lia|done|]. split!; [lia|by simplify_map_eq'].
+  - rewrite /coro_regs_mem_n !lookup_map_seqZ. apply option_eq => ?. case_option_guard; [|done].
+    rewrite !list_lookup_fmap !fmap_Some.
+    setoid_rewrite lookup_take_Some.
+    setoid_rewrite coro_get_regs_lookup_Some.
+    split => ?; destruct_all?; simplify_eq; split!; try lia; rewrite lookup_total_insert_ne // => ?; subst.
+    have /NoDup_alt Hx : NoDup coro_saved_regs by compute_done.
+    efeed pose proof Hx; [exact: Hk| done| ]. lia.
+    have /NoDup_alt Hx : NoDup coro_saved_regs by compute_done.
+    efeed pose proof Hx; [exact: Hk| done| ]. lia.
+Qed.
+
+Lemma coro_regs_mem_n_rs_eq rs1 rs2 n :
+  (∀ i, rs1 !!! i = rs2 !!! i) →
+  coro_regs_mem_n rs1 n = coro_regs_mem_n rs2 n.
+Proof.
+ move => Heq.
+ rewrite /coro_regs_mem_n/coro_get_regs.
+ f_equal. f_equal. f_equal. by apply list_fmap_ext.
+Qed.
+
+Lemma coro_regs_mem_n_0 rs :
+  coro_regs_mem_n rs 0 = ∅.
+Proof. done. Qed.
+Lemma coro_regs_regs_n_0 rs :
+  coro_regs_regs_n rs 0 = ∅.
+Proof. done. Qed.
 
 Definition yield_swap_reg (r : string) (o : Z) : list deep_asm_instr := [
     Aload "R16" "R17" o;
@@ -100,7 +218,8 @@ Definition yield_swap_reg (r : string) (o : Z) : list deep_asm_instr := [
 
 
 Definition yield_asm: gmap Z asm_instr := deep_to_asm_instrs yield_addr (
-  [Amov "R17" coro_state_addr] ++
+  [Amov "R17" coro_state_addr;
+   Amov "R16" 0] ++ (* dummy *)
   mjoin (imap (λ i r, yield_swap_reg r (Z.of_nat i)) (locked saved_registers)) ++ [
   Aload "R16" "R17" (Z.of_nat $ length saved_registers);
   Astore "R30" "R17" (Z.of_nat $ length saved_registers);
@@ -112,6 +231,7 @@ Definition yield_itree : itree (moduleE asm_event (gmap string Z)) unit :=
   ITree.forever (
   '(rs, mem) ← TReceive (λ '(rs, mem), (Incoming, EAJump rs mem));;;
   TAssume (rs !!! "PC" = yield_addr);;;;
+  TAssume (rs !!! "R30" ∉ yield_asm_dom);;;;
   rsold ← TGet;;;
   TAssume (coro_regs_mem rsold ⊆ mem);;;;
   let rs' := (<["PC" := rs !!! "R30"]> rs) in
@@ -130,20 +250,23 @@ Local Ltac go_i :=
   tstep_i; go.
 
 Lemma yield_asm_refines_itree regs :
+  regs !!! "PC" ∉ yield_asm_dom →
   trefines (MS asm_module (initial_asm_state yield_asm))
            (MS (mod_itree _ _) (yield_itree, regs)).
 Proof.
-  apply: tsim_implies_trefines => n0 /=.
-  unshelve eapply tsim_remember. { simpl. exact (λ _ σa '(t, _),
+  move => ?. apply: tsim_implies_trefines => n0 /=.
+  unshelve eapply tsim_remember. { simpl. exact (λ _ σa '(t, rs),
     t ≈ yield_itree ∧
     σa.(asm_cur_instr) = AWaiting ∧
-    σa.(asm_instrs) = yield_asm). }
+    σa.(asm_instrs) = yield_asm ∧
+    rs !!! "PC" ∉ yield_asm_dom). }
   { split!. } { done. }
-  move => n _ Hloop [????] [??] ?. destruct_all?; simplify_eq/=.
-  tstep_i => ????? Hi. simpl.
+  move => n _ Hloop [????] [? rsold] ?. destruct_all?; simplify_eq/=.
+  tstep_i => ?? rs mem ? Hi. simpl.
   tstep_s. rewrite -/yield_itree. go.
   go_s. eexists (_, _). go.
   go_s. split!. go.
+  go_s => ?. go.
   go_s => ?. go.
   go_s.
   go_s => ?. go.
@@ -152,8 +275,171 @@ Proof.
   rewrite /yield_asm deep_to_asm_instrs_cons in Hi. simplify_map_eq.
   tstep_i.
   tstep_i. simplify_map_eq'.
-  (* TODO: finish this proof *)
-Admitted.
+  tstep_i => ??. simplify_map_eq'.
+  rewrite (deep_to_asm_instrs_lookup_nat 1) /=; [|lia].
+  tstep_i.
+  tstep_i. simplify_map_eq'.
+  rename select (itree _ _) into t'.
+  unshelve eapply tsim_remember. { simpl. exact (λ _ σa '(t, rs'),
+    ∃ (n : nat) r16,
+    n ≤ length saved_registers ∧
+    t = t' ∧
+    σa.(asm_cur_instr) = (ARunning []) ∧
+    σa.(asm_regs) = <["PC" := yield_addr + (2 + n * 3)]> $
+                    <["R16" := r16]> $
+                    <["R17" := coro_state_addr]> $
+                    coro_regs_regs_n rsold n ∪ rs ∧
+    σa.(asm_mem) = coro_regs_mem_n rs n ∪ coro_regs_mem rsold ∪ mem ∧
+    σa.(asm_instrs) = yield_asm ∧
+    rs' = <["PC":=rs !!! "R30"]> rs ). }
+  { eexists 0%nat. split!; simplify_map_eq' => //.
+    { apply map_eq => i.
+      destruct (decide (i = "PC")); simplify_map_eq; [f_equal; lia|].
+      destruct (decide (i = "R16")); simplify_map_eq; [done|].
+      destruct (decide (i = "R17")); simplify_map_eq; [done|].
+      by rewrite coro_regs_regs_n_0 left_id_L. }
+   { rewrite coro_regs_mem_n_0 left_id_L. symmetry. by apply map_subseteq_union. } }
+  { done. }
+  move => n1 ? Hloop2 [? rs' ??] [??] [i ?]. destruct_all?. simplify_eq/=.
+  tstep_i => ??. simplify_map_eq'.
+  rewrite (deep_to_asm_instrs_lookup_nat (S (S (i * 3)))) /=; [|lia].
+  have Hlen: length (mjoin (imap (λ (i : nat) (r : string), yield_swap_reg r i) (locked saved_registers))) = 36%nat.
+  { by unlock. }
+  destruct (decide (i = 12%nat)); subst.
+  - repeat match goal with | H : context [take 12 saved_registers] |- _ => rewrite take_ge in H; [|done] end.
+    rewrite lookup_app_r Hlen //=.
+    tstep_i. simplify_map_eq'. split!.
+    tstep_i.
+    tstep_i => ??. simplify_map_eq'.
+    rewrite (deep_to_asm_instrs_lookup_nat (S (S (S (12 * 3))))) /=; [|lia].
+    rewrite lookup_app_r Hlen /=; [|lia].
+    tstep_i. simplify_map_eq'. split!. sort_map_insert. rewrite 2!insert_insert.
+    tstep_i. simplify_map_eq'.
+    tstep_i => ??. simplify_map_eq'.
+    rewrite (deep_to_asm_instrs_lookup_nat (S (S (S (S (12 * 3)))))) /=; [|lia].
+    rewrite lookup_app_r Hlen /=; [|lia].
+    tstep_i. simplify_map_eq'.
+    tstep_i => ??. simplify_map_eq'.
+    rewrite not_elem_of_dom_1.
+    2: { revert select (rsold !!! "PC" ∉ yield_asm_dom). unfold yield_asm_dom. by unlock. }
+    go_s. eexists _. go.
+    go_s. eexists _. go.
+    go_s. split!. {
+      apply map_eq => i.
+      destruct (decide (i = "R16")); simplify_map_eq; [done|].
+      destruct (decide (i = "R17")); simplify_map_eq; [done|].
+      destruct (decide (i = "PC")). 1: by simplify_map_eq.
+      repeat (rewrite lookup_insert_ne; [|done]).
+      destruct (coro_regs_regs rsold !! i) eqn: Heq.
+      * rewrite lookup_union_l // Heq. symmetry. apply lookup_union_Some_l.
+        move: Heq => /coro_regs_regs_lookup_Some[??].
+        apply coro_regs_regs_n_lookup_Some. split!.
+        by rewrite coro_saved_regs_take_PC.
+      * rewrite lookup_union_r // lookup_union_r //.
+        move: Heq => /coro_regs_regs_lookup_None?.
+        apply coro_regs_regs_n_lookup_None. split!.
+        by rewrite coro_saved_regs_take_PC.
+    } {
+      rewrite !insert_union_l.
+      erewrite coro_regs_mem_n_insert; [|done].
+      f_equal.
+      rewrite !lookup_total_alt. rewrite lookup_union_r //.
+      rewrite map_difference_union_r map_difference_empty_dom ?right_id_L //.
+      compute_done.
+    } go.
+    apply: Hloop. { etrans; [|done]. apply ti_le_S. }
+    split!. by simplify_map_eq'.
+  - rewrite lookup_app_l ?Hlen //=.
+    have ->: (i * 3)%nat = (i * 3 + 0)%nat by lia.
+    erewrite join_lookup_Some_same_length_2.
+    2: { apply Forall_forall => ? /elem_of_lookup_imap. naive_solver. }
+    2: { lia. }
+    2: { apply list_lookup_imap_Some. split!. apply list_lookup_lookup_total_lt. unlock => /=. lia. }
+    2: { done. }
+    2: { lia. }
+    simpl.
+    tstep_i. simplify_map_eq'. split!. {
+      apply lookup_union_Some_l. apply lookup_union_Some_raw. right.
+      split.
+      - apply coro_regs_mem_n_lookup_None. lia.
+      - eapply coro_regs_mem_lookup_Some; [done|]. split!; [|lia].
+        apply coro_saved_regs_lookup_saved. lia.
+    } simpl.
+    tstep_i.
+    tstep_i => ??. simplify_map_eq'.
+    rewrite (deep_to_asm_instrs_lookup_nat (S (S (i * 3 + 1)))) /=; [|lia].
+    rewrite lookup_app_l ?Hlen /=; [|lia].
+    erewrite join_lookup_Some_same_length_2.
+    2: { apply Forall_forall => ? /elem_of_lookup_imap. naive_solver. }
+    2: { lia. }
+    2: { apply list_lookup_imap_Some. split!. apply list_lookup_lookup_total_lt. unlock => /=. lia. }
+    2: { done. }
+    simpl.
+    tstep_i. simplify_map_eq'. split!. {
+      apply lookup_union_Some_l. apply lookup_union_Some_raw. right.
+      split.
+      - apply coro_regs_mem_n_lookup_None. lia.
+      - eapply coro_regs_mem_lookup_Some; [done|]. split!; [|lia].
+        apply coro_saved_regs_lookup_saved. lia.
+    } simpl. unlock.
+    tstep_i. simplify_map_eq'.
+    rewrite lookup_total_insert_ne.
+    2: { do 12 (destruct i as [|i]; try done). }
+    rewrite lookup_total_insert_ne.
+    2: { do 12 (destruct i as [|i]; try done). }
+    tstep_i => ??. simplify_map_eq'.
+    rewrite (deep_to_asm_instrs_lookup_nat (S (S (i * 3 + 2)))) /=; [|lia].
+    rewrite lookup_app_l ?Hlen /=; [|lia].
+    erewrite join_lookup_Some_same_length_2.
+    2: { apply Forall_forall => ? /elem_of_lookup_imap. naive_solver. }
+    2: { lia. }
+    2: { apply list_lookup_imap_Some. split!. apply list_lookup_lookup_total_lt. unlock => /=. lia. }
+    2: { done. }
+    simpl. unlock.
+    tstep_i. simplify_map_eq'.
+    tstep_i. rewrite lookup_total_insert_ne.
+    2: { do 12 (destruct i as [|i]; try done). }
+    simplify_map_eq'.
+    apply: Hloop2; [done|]. eexists (i + 1)%nat. split!.
+    + lia.
+    + sort_map_insert. rewrite !insert_insert. apply map_eq => j.
+      destruct (decide (j = "PC")); simplify_map_eq; [f_equal; lia|].
+      rewrite (lookup_insert_ne _ "PC"); [|done].
+      destruct (decide (j = (saved_registers !!! i))); simplify_map_eq. {
+        rewrite lookup_insert_ne.
+        2: { do 12 (destruct i as [|i]; try done). }
+        rewrite lookup_insert_ne.
+        2: { do 12 (destruct i as [|i]; try done). }
+        symmetry. apply lookup_union_Some_l.
+        apply coro_regs_regs_n_lookup_Some. split!.
+        apply elem_of_take. eexists i. split; [|lia].
+        apply coro_saved_regs_lookup_saved. lia.
+      }
+      destruct (decide (j = "R16")); simplify_map_eq; [done|].
+      destruct (decide (j = "R17")); simplify_map_eq; [done|].
+      destruct (coro_regs_regs_n rsold i !! j) eqn: Heq.
+      * rewrite lookup_union_l // Heq. symmetry. apply lookup_union_Some_l.
+        move: Heq => /coro_regs_regs_n_lookup_Some[??].
+        apply coro_regs_regs_n_lookup_Some. split!.
+        rewrite coro_saved_regs_take_saved; [done|lia|done].
+      * rewrite lookup_union_r // lookup_union_r //.
+        move: Heq => /coro_regs_regs_n_lookup_None?.
+        apply coro_regs_regs_n_lookup_None. split!.
+        rewrite coro_saved_regs_take_saved; [done|lia|done].
+    + rewrite lookup_total_insert_ne.
+      2: { do 12 (destruct i as [|i]; try done). }
+      rewrite lookup_total_insert_ne.
+      2: { do 12 (destruct i as [|i]; try done). }
+      rewrite lookup_total_insert_ne.
+      2: { do 12 (destruct i as [|i]; try done). }
+      rewrite !insert_union_l.
+      erewrite coro_regs_mem_n_insert. 2: { apply coro_saved_regs_lookup_saved. lia. }
+      f_equal. f_equal. apply coro_regs_mem_n_rs_eq => k.
+      destruct (decide (k = saved_registers !!! i)); simplify_map_eq' => //.
+      rewrite !lookup_total_alt. rewrite lookup_union_r //.
+      apply coro_regs_regs_n_lookup_None.
+      do 12 (destruct i as [|i]; [compute_done|]). lia.
+Qed.
 
 Inductive coro_prod_filter_state :=
 | CPFInit
@@ -295,7 +581,10 @@ Proof.
   }
   have Hf1in : ∀ f i1 i2, f2i1 !! f  = Some i1 → f2i !! f = Some i2 → i1 = i2.
   { move => ???. rewrite /f2i lookup_union_Some_raw. naive_solver. }
-  etrans. { apply: asm_prod_trefines; [|done]. apply (yield_asm_refines_itree regs_init). }
+  etrans. {
+    apply: asm_prod_trefines; [|done]. apply (yield_asm_refines_itree regs_init).
+    fast_set_solver.
+  }
   apply: tsim_implies_trefines => n0 /=.
   tstep_i => *. case_match; destruct_all?; simplify_eq/=.
   tstep_s. split!.
@@ -385,7 +674,7 @@ Proof.
     all: apply: steps_spec_step_end; [done|] => σ'' ?; assert (σ'' = σ') by naive_solver.
     + (* left to right *)
       tstep_s => ?.
-      tstep_i => *. destruct_all?; simplify_map_eq'.
+      tstep_i => *. unfold i2a_regs_call in *. destruct_all?; simplify_map_eq'.
       rewrite bool_decide_false. 2: fast_set_solver.
       rewrite bool_decide_false. 2: fast_set_solver.
       move => /= *. destruct_all?; simplify_map_eq'.
@@ -394,6 +683,7 @@ Proof.
       go_i => -[??]. go.
       go_i => ?. simplify_eq. go.
       go_i. split; [done|]. go.
+      go_i. split; [fast_set_solver|]. go.
       go_i.
       iSatStart. iIntros!. revert select (x1 ⊣⊢ _) => ->. iDestruct!.
       iDestruct select (i2a_mem_inv _ _ _) as "Hm".
@@ -434,7 +724,7 @@ Proof.
         tstep_s. eexists (Some (Incoming, _)). split!. apply: steps_spec_step_end; [done|] => ??. tend. split!; [done|].
         apply: Hloop. { etrans; [|done]. etrans; [|done]. apply ti_le_S. }
         split!.
-        { simplify_map_eq'. revert select (i2a_regs_call _ _) => ->. done. }
+        { simplify_map_eq'. done. }
         { apply map_preserved_insert_r_not_in; [compute_done|]. done. }
         { etrans; [done|]. etrans; [done|].
           apply map_scramble_insert_r_in; [compute_done|].
@@ -463,7 +753,7 @@ Proof.
         tstep_s. eexists (Some (Incoming, _)). split!. apply: steps_spec_step_end; [done|] => ??. tend. split!; [done|].
         apply: Hloop. { etrans; [|done]. etrans; [|done]. apply ti_le_S. }
         split!.
-        { simplify_map_eq'. revert select (i2a_regs_call _ _) => ->. done. }
+        { simplify_map_eq'. done. }
         { apply map_preserved_insert_r_not_in; [compute_done|]. done. }
         { etrans; [done|]. etrans; [done|].
           apply map_scramble_insert_r_in; [compute_done|].
@@ -554,7 +844,7 @@ Proof.
     all: apply: steps_spec_step_end; [done|] => σ'' ?; assert (σ'' = σ') by naive_solver.
     + (* right to left *)
       tstep_s => ?.
-      tstep_i => *. destruct_all?; simplify_map_eq'.
+      tstep_i => *. unfold i2a_regs_call in *. destruct_all?; simplify_map_eq'.
       rewrite bool_decide_false. 2: fast_set_solver.
       rewrite bool_decide_false. 2: fast_set_solver.
       move => /= *. destruct_all?; simplify_map_eq'.
@@ -563,6 +853,7 @@ Proof.
       go_i => -[??]. go.
       go_i => ?. simplify_eq. go.
       go_i. split; [done|]. go.
+      go_i. split; [fast_set_solver|]. go.
       go_i.
       iSatStart. iIntros!. revert select (x2 ⊣⊢ _) => ->. iDestruct!.
       iDestruct select (i2a_mem_inv _ _ _) as "Hm".
@@ -607,7 +898,7 @@ Proof.
         apply map_scramble_insert_r_in; [compute_done|].
         by apply coro_regs_regs_touched_scramble. }
       { simplify_map_eq'. iSplit; iIntros!; iFrame. }
-      { simplify_map_eq'. revert select (i2a_regs_call _ _) => ->. done. }
+      { simplify_map_eq'. done. }
       { apply map_preserved_insert_r_not_in; [compute_done|]. done. }
       { unfold i2a_regs_call in *. simplify_map_eq'. done. }
     + (* right call to outside *)
